tuning
* CDCL_Two_Watched_Literals_List_Conflict_Assn ~> CDCL_Two_Watched_Literals_Lookup_Conflict
* remove comments
* remove unused functions
* give name to functions for more readable code SML
* moving some theorems and definitions

Weidenbach_Book/Array_UInt.thy
@@ -198,5 +198,11 @@ lemma array_set_hnr_u[sepref_fr_rules]:
       heap_array_set_u_def Array.upd'_def
      nat_of_uint32_code[symmetric])
 
+definition (in -)length_aa_u :: \<open>('a::heap array_list) array \<Rightarrow> uint32 \<Rightarrow> nat Heap\<close> where
+  \<open>length_aa_u xs i = length_aa xs (nat_of_uint32 i)\<close>
+
+lemma length_aa_u_hnr[sepref_fr_rules]: \<open>(uncurry length_aa_u, uncurry (RETURN \<circ>\<circ> length_ll)) \<in>
+     [\<lambda>(xs, i). i < length xs]\<^sub>a (arrayO_assn (arl_assn R))\<^sup>k *\<^sub>a uint32_nat_assn\<^sup>k \<rightarrow> nat_assn\<close>
+  by sepref_to_hoare (sep_auto simp: uint32_nat_rel_def length_aa_u_def br_def)
 
 end
